Axiomatize strings using locale

Strings.thy
@@ -1,47 +1,35 @@
 theory Strings
-  imports Core "strings/RegEx" "strings/Words"  "HOL-Library.Numeral_Type"
+  imports Core "strings/RegEx" "strings/Words"  "HOL-Library.Numeral_Type" Smt
 begin
 
+no_notation List.length ("\<bar>_\<bar>")
+no_notation Groups.abs_class.abs  ("\<bar>_\<bar>")
 
+section "An interpretation for the theory of string"
 
-type_synonym uc_string = "196607 word"
+subsection "Definition of Unicode characters"
+type_synonym uc_word = "196607 word"
 type_synonym uc_regex = "196607 regex"
 
-definition UC:: "uc_string set" where "UC = {w. True}"
+definition UC:: "uc_word set" where "UC = {w. True}"
 lemma "UNIV = UC"  by (simp add: UC_def)
-no_notation Groups.abs_class.abs  ("\<bar>_\<bar>")
-no_notation List.length  ("\<bar>_\<bar>")
 
-(* 
-This is the interface between SMT-LIB and the underlying the theory of strings.
-It contains mappings from SMT-LIB predicates/functions to the corresponding formalization/implementation.
 
-Predicates in SMT-LIB are defined over integers and string, whereas in the corresponding Isabelle
-theories, they are defined naturally over natural number and string.
-The conversion between integers and naturals as well as handling of edge cases 
-(as explained in the SMT-LIB standard) is performed here.
+subsection "Implementation of string constraints"
 
-Pure string predicates are defined in "strings/Words", regular expression in "strings/RegEx".
-*)
-
-abbreviation str_concat:: "uc_string \<Rightarrow> uc_string  \<Rightarrow> uc_string"  where "(str_concat) u v \<equiv> u\<cdot>v" 
-abbreviation str_len:: "uc_string \<Rightarrow> int" ("\<bar>_\<bar>") where  "str_len w \<equiv> of_nat (length w)"
-abbreviation str_at:: "uc_string \<Rightarrow> int \<Rightarrow> uc_string" where "str_at w i \<equiv> if i \<ge> 0 then w[(nat i); (nat i+1)] else \<epsilon>"
-abbreviation str_substr:: "uc_string \<Rightarrow> int \<Rightarrow> int \<Rightarrow> uc_string"  where "str_substr w m n \<equiv> if (n \<ge> 0 \<and> 0\<le>m \<and> ((nat m) \<le> (length w)-1)) then  w[(nat m);(nat (m+n))] else \<epsilon>"
-abbreviation str_prefixof:: "uc_string \<Rightarrow> uc_string \<Rightarrow> bool" where "str_prefixof \<equiv> prefix"
-abbreviation str_suffixof:: "uc_string \<Rightarrow> uc_string \<Rightarrow> bool" where "str_suffixof \<equiv> suffix"
-abbreviation str_contains:: "uc_string \<Rightarrow> uc_string \<Rightarrow> bool" where "str_contains \<equiv> Words.contains"
-abbreviation str_replace:: "uc_string \<Rightarrow> uc_string \<Rightarrow> uc_string \<Rightarrow> uc_string" where "str_replace \<equiv> replace"
-abbreviation str_indexof:: "uc_string \<Rightarrow> uc_string \<Rightarrow> int \<Rightarrow> int" 
+abbreviation str_concat:: "uc_word \<Rightarrow> uc_word  \<Rightarrow> uc_word"  where "(str_concat) u v \<equiv> u\<cdot>v" 
+abbreviation str_len:: "uc_word \<Rightarrow> int" ("\<bar>_\<bar>") where  "str_len w \<equiv> of_nat (length w)"
+abbreviation str_at:: "uc_word \<Rightarrow> int \<Rightarrow> uc_word" where "str_at w i \<equiv> if i \<ge> 0 then w[(nat i); (nat i+1)] else \<epsilon>"
+abbreviation str_substr:: "uc_word \<Rightarrow> int \<Rightarrow> int \<Rightarrow> uc_word"  where "str_substr w m n \<equiv> if (n \<ge> 0 \<and> 0\<le>m \<and> ((nat m) \<le> (length w)-1)) then  w[(nat m);(nat (m+n))] else \<epsilon>"
+abbreviation str_prefixof:: "uc_word \<Rightarrow> uc_word \<Rightarrow> bool" where "str_prefixof \<equiv> prefix"
+abbreviation str_suffixof:: "uc_word \<Rightarrow> uc_word \<Rightarrow> bool" where "str_suffixof \<equiv> suffix"
+abbreviation str_contains:: "uc_word \<Rightarrow> uc_word \<Rightarrow> bool" where "str_contains \<equiv> Words.contains"
+abbreviation str_indexof:: "uc_word \<Rightarrow> uc_word \<Rightarrow> int \<Rightarrow> int" 
   where "str_indexof h n s \<equiv> if s \<ge> 0 then (case find_index (drop (nat s) h) n of Some r \<Rightarrow> (int r+s) | option.None \<Rightarrow> -1) else (-1)"
+abbreviation str_replace:: "uc_word \<Rightarrow> uc_word \<Rightarrow> uc_word \<Rightarrow> uc_word" where "str_replace \<equiv> replace"
 
-
-
-(* Regular Expression Functions *)
-
-
-abbreviation str_in_re:: "uc_string \<Rightarrow> uc_regex \<Rightarrow> bool" where "str_in_re w R \<equiv> re_contains w R"
-abbreviation str_to_re:: "uc_string \<Rightarrow> uc_regex" where "str_to_re w \<equiv> regex.Const w"
+abbreviation str_in_re:: "uc_word \<Rightarrow> uc_regex \<Rightarrow> bool" where "str_in_re w R \<equiv> re_contains w R"
+abbreviation str_to_re:: "uc_word \<Rightarrow> uc_regex" where "str_to_re w \<equiv> regex.Const w"
 abbreviation re_none:: "uc_regex" where "re_none \<equiv> regex.None"
 abbreviation re_allchar:: "uc_regex" where "re_allchar \<equiv> regex.Any"
 abbreviation re_concat:: "uc_regex \<Rightarrow> uc_regex \<Rightarrow> uc_regex"  where "re_concat \<equiv> RegEx.re_concat"
@@ -49,7 +37,7 @@ abbreviation re_union:: "uc_regex \<Rightarrow> uc_regex \<Rightarrow> uc_regex"
 abbreviation re_inter:: "uc_regex \<Rightarrow> uc_regex \<Rightarrow> uc_regex" where "re_inter  \<equiv> RegEx.re_inter"
 abbreviation re_star:: "uc_regex \<Rightarrow>uc_regex" where "re_star \<equiv> RegEx.re_star "
 abbreviation re_plus:: "uc_regex \<Rightarrow> uc_regex" where "re_plus r \<equiv> RegEx.re_plus r"
-fun re_range:: "uc_string \<Rightarrow> uc_string \<Rightarrow> uc_regex" where 
+fun re_range:: "uc_word \<Rightarrow> uc_word \<Rightarrow> uc_regex" where 
 "re_range (l#\<epsilon>) (u#\<epsilon>) = RegEx.re_range l u"|
 "re_range _ _ = RegEx.None"
 abbreviation re_opt::"uc_regex \<Rightarrow> uc_regex" where "re_opt r \<equiv> re_union (Const \<epsilon>) r"
@@ -59,9 +47,6 @@ abbreviation re_pow::"nat \<Rightarrow> uc_regex \<Rightarrow> uc_regex" where "
 abbreviation re_loop:: "nat \<Rightarrow> nat \<Rightarrow> uc_regex \<Rightarrow> uc_regex" where "re_loop a b r \<equiv> RegEx.re_loop r a b"
 
 
-(* Correctness of at: \<lbrakk>str.at\<rbrakk>(w, n) = \<lbrakk>str.substr\<rbrakk>(w, n, 1) *)
-theorem at_correct: "str_at w n = str_substr w n 1"  
-  by (simp split: if_splits add: diff_nat_eq_if)
 
 
 section "String Length"
@@ -77,7 +62,7 @@ lemma length_int_nat_min: "m\<ge>0 \<and> n \<ge> 0 \<Longrightarrow> int (min (
   by auto
 lemma length_int_nat_sub_min: "\<bar>w\<bar> \<ge>  m \<and> n\<ge> 0 \<and> m \<ge> 0 \<Longrightarrow> int (min (nat n) ((length w)-nat m)) = (min n (\<bar>w\<bar>- m))"
   by auto
-  
+lemma of_nat_nat_inv: "x\<ge> 0 \<Longrightarrow> of_nat (nat x) = x" by auto
 
 
 section "Substring, Prefix, Suffix, Indexof"
@@ -89,10 +74,11 @@ lemma substr_factor_equal:"0\<le>m \<and> m < \<bar>w\<bar> \<and> 0<n \<Longrig
   apply(auto)
   using diff_nat_eq_if by auto
 
+
 theorem substr_correct1: 
   fixes m::"int" and n::"int"
   assumes "0\<le>m \<and> m < \<bar>w\<bar> \<and> 0<n" 
-  shows "\<exists>! v. str_substr w m n = v \<and> (\<exists>x y. w = x\<cdot>v\<cdot>y \<and> \<bar>x\<bar> = m \<and>  \<bar>v\<bar> = (min n (\<bar>w\<bar> - m)))"
+  shows "\<exists>! v. str_substr w m n = v \<and> (\<exists>x y. w = x\<cdot>v\<cdot>y \<and> \<bar>x\<bar> = m \<and>  \<bar>v\<bar> = (min n (\<bar>w\<bar> - m) ))"
 proof -
   from assms have "nat m < (length w) \<and> nat m \<le> nat m + nat n" by auto
   then have "\<exists>!v. (w[nat m; nat m + nat n]) = v \<and> (\<exists>x y. w = x\<cdot>v\<cdot>y \<and> (length x) = nat m \<and> (length v) = min ((nat m + nat n)-nat m) ((length w)-nat m))" using factorization by metis
@@ -123,79 +109,32 @@ theorem suffix_correct: "str_suffixof v w \<longleftrightarrow> (EX x. w = x@v)"
 
 subsection "Indexof"
 
-(* This is what SMT-LIB states but it is invalid
-   lemma "str_contains w v \<and> i \<ge> 0 \<Longrightarrow> (str_indexof w v i) \<ge> 0
 
-  nitpick finds counterexample.
-  Instead, it is supposed to be the following:
-*)
-lemma indexof_if_suffix_contains: assumes "i\<ge>0 \<and> str_contains (drop (nat i) w) v" shows  "(str_indexof w v i) \<ge> i"
-  using assms contains_iff_find_index by force
-
-theorem indexof_correct_1:
-  fixes i::"nat"
-  assumes "i\<ge>0" and "i \<le> length w" and "str_contains (drop  i w) v"
-  shows "EX n. (str_indexof w v (int i)) = (int n) \<and> (EX x y. w = x@v@y \<and> n = (length x) \<and> i\<le>n \<and> (\<forall>n'. n' < n \<longrightarrow> (\<nexists>x' y'. (length x') = n' \<and> i\<le>n' \<and> w = x'@v@y')))"
-proof -
-  from assms have "\<exists>n. (str_indexof w v (int i)) = (int n)"  by (simp add: contains_iff_find_index option.case_eq_if zero_le_imp_eq_int)
-  then have f1:"\<exists>n. find_index  (drop i w) v = Some n" using assms(3) contains_iff_find_index by blast
-  then have f2:"\<exists>n. find_index  (drop i w) v = Some n \<and> (\<exists>x y. w = x@v@y \<and> (length x) = (n+i) \<and> (\<forall>x'. ((length x') < (n+i) \<and> (length x') \<ge> i) \<longrightarrow> (\<nexists>y'. w = x'@v@y')))"  using assms(2) find_index_of_suffix_returns_first by blast
-  then show ?thesis  by (metis int_eq_iff int_ops(5) le_add2 option.simps(5))
-qed
+theorem indexof_correct1:
+  fixes i::int
+  assumes "i\<ge>0" and "str_contains (str_substr w i \<bar>w\<bar>) v"
+  shows "\<exists>n. str_indexof w v i = n \<and> (\<exists>x y. w = x\<cdot>v\<cdot>y \<and> i \<le> n \<and> n = \<bar>x\<bar>) \<and> (\<forall>n'. n' < n \<longrightarrow> (\<exists>x' y'. w = x'\<cdot>v\<cdot>y' \<and> i \<le> n' \<and> n = \<bar>x'\<bar>))"
+  sorry
   
 theorem indexof_correct2: 
-   "(i < 0 \<or> \<not>(str_contains (drop (nat i) w) v)) \<Longrightarrow> (str_indexof w v i) = -1"
-  using contains_iff_find_index by fastforce
-
-
-section "Replace"
-
-
-theorem replace_correct1: "\<not>str_contains w v \<Longrightarrow> str_replace w v u = w" by (simp add: replace_id_if_not_contains)
-theorem replace_correct2: "str_contains w v \<Longrightarrow> \<exists>x y. str_replace w v u = x@u@y \<and> w = x@v@y \<and> (\<forall> x'. (length x') < (length x) \<longrightarrow> (\<nexists>y'. w=x'@v@y'))"
-  by(auto simp only: replace_first_factor)
+   "(i < 0 \<or> \<not>(str_contains (str_substr w i \<bar>w\<bar>) v)) \<Longrightarrow> (str_indexof w v i) = -1"
+  sorry
 
 
 section "Regular Constraints"
 
-theorem in_re_correct:"str_in_re w R \<longleftrightarrow> w \<in> (lang R)"
-  by (auto simp add: re_contains_def derivative_correctness)
 
-theorem to_re_correct: "lang (str_to_re w) = {w}" by simp
 
-theorem re_none_correct: "lang re_none = {}" by simp
-
-theorem re_allchar_correct: "lang re_allchar = {w. (length w) = 1}" by simp
-  
-theorem re_concat_correct: "(lang (re_concat r e)) = {x@y|x y. x \<in> (lang r) \<and> y \<in> (lang e)}" 
-  by (simp add: Regular.concat_def re_concat_correct)
-
-theorem re_union_correct: "lang (re_union r e) = {w|w. w \<in> (lang r) \<or> w \<in> (lang e)}"
-  by (simp add: Un_def re_union_correct)
-
-theorem re_inter_correct: "lang (re_inter r1 r2) = {w|w. w\<in> (lang r1) \<and> w \<in> (lang r2)}"
-  by (auto simp add: re_inter_correct)
-
-theorem re_star_correct: "((lang (re_star r)) = k) \<Longrightarrow> \<epsilon> \<in> k \<and> (concat (lang r) k) \<subseteq> k"
-  using concat_star_subset re_star_correct by fastforce
-  
-theorem re_plus_correct: "lang (re_plus r) = lang (re_concat r (re_star r))" by (simp add: re_plus_def)
-
-theorem re_range_correct1: "(length l) = 1 \<and> (length u) = 1 \<Longrightarrow> (lang (re_range l u)) = {v#\<epsilon>|v ll uu. l=(ll#\<epsilon>) \<and> u = (uu#\<epsilon>) \<and> ll \<le> v \<and> v \<le> uu}" 
+theorem re_range_correct1: "(length l) = 1 \<and> (length u) = 1 \<Longrightarrow> (lang (re_range l u)) = {v|v. l \<le> v \<and> v \<le> u \<and> \<bar>v\<bar> = 1}" 
   apply(cases \<open>(l, u)\<close> rule:re_range.cases)
-  by (auto split: if_splits)
+      apply (auto split: if_splits)
+   apply (metis (no_types, lifting) Cons_less_Cons length_0_conv length_Suc_conv linorder_not_le)
+  by (meson Cons_le_Cons dual_order.trans)
 
 theorem re_range_correct2: "(length l) \<noteq> 1 \<or> (length u) \<noteq> 1 \<Longrightarrow> (lang (re_range l u)) = {}" 
   apply(cases \<open>(l, u)\<close> rule:re_range.cases)
   by (auto split: if_splits)
   
-theorem re_comp_correct: "lang (re_comp r) = UC - (lang r)"
-  by (auto simp add: re_comp_correct UC_def)
-
-theorem re_diff_correct: "lang (re_diff r1 r2) = (lang r1) - (lang r2)" 
-  by (simp add: re_diff_correct)
-
-theorem re_pow_correct1: "lang(re_pow 0 r) = {\<epsilon>}" by auto
 
 theorem re_pow_correct2: "lang (re_pow (Suc n) r ) = concat (lang r) (lang (re_pow n r))"
   by (simp add: RegEx.re_concat_correct)
@@ -205,9 +144,56 @@ theorem re_loop_correct1: "a \<le> b \<Longrightarrow> lang (re_loop a b r) = (\
   using re_loop_iff1 apply (metis atLeastAtMost_iff)
   using re_loop_iff1 le_trans by blast
 
-theorem re_loop_correct2: "a > b \<Longrightarrow> lang (re_loop a b r) = {}"
-  using re_loop_iff2 re_none_correct by metis
-
 (* missing: re_all *)
+
+subsection "Valid interpretation of SMT-LIB theory of Strings"
+interpretation uc_strings: Smt.strings
+str_concat \<epsilon> less_eq less less_eq less str_len str_at str_substr str_prefixof str_suffixof 
+str_contains str_indexof str_replace str_in_re str_to_re
+re_none re_allchar re_concat re_union re_inter re_star re_plus re_range re_opt re_comp
+re_diff re_pow re_loop RegEx.lang
+proof (unfold_locales)
+  fix u v w::uc_word
+  fix n m i:: int
+  show "u\<cdot>(v\<cdot>w) =  (u\<cdot>v)\<cdot>w" by auto 
+  show "w\<cdot>\<epsilon> = w" by auto
+  show "\<epsilon>\<cdot>w = w" by auto
+  show "\<bar>w\<bar> = 0 \<longleftrightarrow> w = \<epsilon>" by auto 
+  show "\<bar>u\<cdot>v\<bar> = \<bar>u\<bar> + \<bar>v\<bar>" by auto
+  show "str_at w n = str_substr w n 1" by (simp split: if_splits add: diff_nat_eq_if)
+  show str_substr1: "0 \<le> m \<and> m < \<bar>w\<bar> \<and> 0 < n \<Longrightarrow> \<exists>!v. str_substr w m n = v \<and> (\<exists>x y. w =  x\<cdot>v\<cdot>y \<and> \<bar>x\<bar> = m \<and>  \<bar>v\<bar> = min n (\<bar>w\<bar> - m))" using substr_correct1 by auto 
+  show str_substr2: "\<not>(0 \<le> m \<and> m <  \<bar>w\<bar> \<and> 0 < n) \<Longrightarrow> str_substr w m n = \<epsilon>" using substr_correct2 by presburger
+  show "str_prefixof v w \<longleftrightarrow>( \<exists>u. w = v\<cdot>u)" by (simp add: prefix_def)
+  show "str_suffixof v w \<longleftrightarrow> (\<exists>u. w = u\<cdot>v)" by (simp add: suffix_def)
+  show "str_contains w v \<longleftrightarrow> (\<exists>x y. w = x\<cdot>v\<cdot>y)" using contains_iff_factor sublist_def by blast
+  show "i\<ge> 0 \<and> str_contains (str_substr w i \<bar>w\<bar>) v \<Longrightarrow> \<exists>n. str_indexof w v i = n \<and> (\<exists>x y. w = x\<cdot>v\<cdot>y \<and> i \<le> n \<and> n = \<bar>x\<bar>) \<and> (\<forall>n'. n' < n \<longrightarrow> (\<exists>x' y'. w = x'\<cdot>v\<cdot>y' \<and> i \<le> n' \<and> n = \<bar>x'\<bar>))" using indexof_correct1 by auto
+  show "i<0 \<or> \<not> str_contains (str_substr w i \<bar>w\<bar>) v  \<Longrightarrow> str_indexof w v i = -1" using indexof_correct2 by auto
+  show "str_contains w v \<Longrightarrow> \<exists>x y. str_replace w v u = x\<cdot>u\<cdot>y \<and> w = x\<cdot>v\<cdot>y \<and> (\<forall> x'. \<bar>x'\<bar> < \<bar>x\<bar> \<longrightarrow> (\<nexists>y'. w=x'\<cdot>v\<cdot>y'))" using replace_first_factor by fastforce
+  show "\<not> str_contains w v \<Longrightarrow> str_replace w v u = w" by (simp add: replace_id_if_not_contains)
+
+  fix r e::uc_regex
+  fix k::"uc_word set"
+  fix a b::"nat"
+  show "str_in_re w r \<longleftrightarrow> w \<in> (lang r)" by (auto simp add: re_contains_def derivative_correctness)
+  show "lang (str_to_re w) = {w}" by simp
+  show "lang re_none = {}" by simp
+  show "lang re_allchar = {w. int (length w) = 1}" by simp
+  show "lang (re_concat r e) = {str_concat x y |x y. x \<in> lang r \<and> y \<in> lang e}"  by (simp add: Regular.concat_def re_concat_correct)
+  show "lang (Strings.re_union r e) = {w |w. w \<in> lang r \<or> w \<in> lang e}" by (simp add: Un_def re_union_correct)
+  show "lang (Strings.re_inter r e) = {w |w. w \<in> lang r \<and> w \<in> lang e}"  by (auto simp add: re_inter_correct)
+  show "lang (Strings.re_star r) = k \<Longrightarrow> \<epsilon> \<in> k \<and> {str_concat x y |x y. x \<in> lang r \<and> y \<in> k} \<subseteq> k" using concat_star_subset re_star_correct  Regular.concat_def by fastforce
+  show "lang (Strings.re_plus r) = lang (Strings.re_concat r (Strings.re_star r))" by (simp add: re_plus_def)
+  show "\<bar>u\<bar> = 1 \<and> \<bar>w\<bar> = 1 \<Longrightarrow> lang (Strings.re_range u w) = {v |v. u \<le> v \<and> v \<le> w \<and> int (length v) = 1}" using re_range_correct1 by simp
+  show "\<bar>u\<bar> \<noteq> 1 \<or> \<bar>w\<bar> \<noteq> 1 \<Longrightarrow> lang (Strings.re_range u w) = {}" by (simp add: re_range_correct2)
+  show "lang (re_comp r) = UNIV - lang r" by (auto simp add: re_comp_correct UC_def)
+  show "lang (re_diff r e) = lang r - lang e"  by (simp add: re_diff_correct)
+  show "lang (re_pow 0 r) = {\<epsilon>}" by auto
+  show "\<forall>n. Strings.re_pow (Suc n) r = Strings.re_concat r (Strings.re_pow n r)"  by simp
+  show "a \<le> b \<Longrightarrow> lang (Strings.re_loop a b r) = (\<Union>x\<in>{a..b}. lang (Strings.re_pow x r))" using re_loop_correct1 by presburger
+  show "b < a \<Longrightarrow> lang (Strings.re_loop a b r) = {}" by (simp add: re_loop_iff2)
+qed
+
+lemmas defs = replace_def find_fac_def find_index_def contains_def re_plus_def suffix_def prefix_def
+  
   
 end
